defined custom induction scheme for eager_eval_expr, still needs a bit of tweaking

src/EagerEvalInd.v
@@ -1,20 +1,20 @@
-Require Import Eager.
 Require Import AST.
 Require Import List.
 Require Import Semantics.
 Require Import String.
 Require Import Builtins.
+Require Import Eager.
 
-Print eager_eval_expr_ind.
 
-Print eager_eval_expr.
 
 Definition eager_eval_expr_ind_total 
   (P : genv -> tenv -> senv -> Expr -> strictval -> Prop)
   (Pl : genv -> tenv -> senv -> list Expr -> list strictval -> Prop)
   (HTuple : forall (ge : genv) (TE : tenv) (E : senv) (l : list Expr)
                    (vs : list strictval),
-      Forall2 (eager_eval_expr ge TE E) l vs -> P ge TE E (ETuple l) (stuple vs))
+      Forall2 (eager_eval_expr ge TE E) l vs ->
+      Pl ge TE E l vs ->
+      P ge TE E (ETuple l) (stuple vs))
   (HTupleSel : forall (ge : genv) (TE : tenv) (E : senv) (e : Expr) 
                       (l : list strictval) (n : nat) (v : strictval),
       eager_eval_expr ge TE E e (stuple l) ->
@@ -36,12 +36,12 @@ Definition eager_eval_expr_ind_total
                       (erase_decl_groups decls E) expr v ->
       P (bind_decl_groups decls ge) TE (erase_decl_groups decls E) expr v ->
       P ge TE E (EWhere expr decls) v)
-  (HIf : forall (ge : genv) (TE : tenv) (E : senv) (c t f4 : Expr) 
+  (HIf : forall (ge : genv) (TE : tenv) (E : senv) (c t f : Expr) 
                 (v : strictval) (b : bool),
       eager_eval_expr ge TE E c (sbit b) ->
       P ge TE E c (sbit b) ->
-      eager_eval_expr ge TE E (if b then t else f4) v ->
-      P ge TE E (if b then t else f4) v -> P ge TE E (EIf c t f4) v)
+      eager_eval_expr ge TE E (if b then t else f) v ->
+      P ge TE E (if b then t else f) v -> P ge TE E (EIf c t f) v)
   (HLocalVar : forall (ge : genv) (TE : tenv) (E : ident -> option strictval) 
                       (id : ident) (v : strictval), E id = Some v -> P ge TE E (EVar id) v)
   (HGlobalVar : forall (ge : genv) (TE : tenv) (E : ident -> option strictval) 
@@ -53,15 +53,15 @@ Definition eager_eval_expr_ind_total
         P ge TE E (EAbs id exp) (sclose id exp TE E))
   (HTAbs : forall (ge : genv) (TE : tenv) (E : senv) (e : Expr) (id : ident),
         P ge TE E (ETAbs id e) (stclose id e TE E))
-  (HApp : forall (ge : genv) (TE : tenv) (E : senv) (f9 : Expr) 
+  (HApp : forall (ge : genv) (TE : tenv) (E : senv) (f : Expr) 
           (id : ident) (exp : Expr) (E' : ident -> option strictval)
           (TE' : ident -> option Tval) (a : Expr) (av v : strictval),
-        eager_eval_expr ge TE E f9 (sclose id exp TE' E') ->
-        P ge TE E f9 (sclose id exp TE' E') ->
+        eager_eval_expr ge TE E f (sclose id exp TE' E') ->
+        P ge TE E f (sclose id exp TE' E') ->
         eager_eval_expr ge TE E a av ->
         P ge TE E a av ->
         eager_eval_expr ge TE' (extend E' id av) exp v ->
-        P ge TE' (extend E' id av) exp v -> P ge TE E (EApp f9 a) v)
+        P ge TE' (extend E' id av) exp v -> P ge TE E (EApp f a) v)
   (HTApp : forall (ge : genv) (TE : tenv) (TE' : ident -> option Tval) 
            (E : senv) (e : Expr) (id : ident) (e' : Expr)
            (E' : ident -> option strictval) (v : strictval) 
@@ -102,23 +102,144 @@ Definition eager_eval_expr_ind_total
   (E : senv)
   (expr : Expr)
   (v : strictval)
-  (eval : eager_eval_expr ge TE E expr v) : P ge TE E expr v .
-Admitted.
-(*  let fix go ge E exp v eval : P ge E exp v :=
-      let fix go_list ge E es vs f2eval : Pl ge E es vs :=
-          match f2eval in (Forall2 _ es0 vs0) return (Pl ge E es0 vs0) with
-          | Forall2_nil => HPlnil ge E
+  (eval : eager_eval_expr ge TE E expr v) : P ge TE E expr v  :=
+  let fix go ge TE E exp v eval : P ge TE E exp v :=
+      let fix go_list ge TE E es vs f2eval : Pl ge TE E es vs :=
+          match f2eval in (Forall2 _ es0 vs0) return (Pl ge TE E es0 vs0) with
+          | Forall2_nil => HPlnil ge TE E
           | Forall2_cons e' v' es' vs' eval_fst forall_eval_rest =>
-            HPlcons ge E e' v' es' vs' (go ge E e' v' eval_fst) (go_list ge E es' vs' forall_eval_rest)
+            HPlcons ge TE E e' v' es' vs' (go ge TE E e' v' eval_fst) (go_list ge TE E es' vs' forall_eval_rest)
           end
-          in
-      match eval in (eager_eval_expr ge0 E0 exp0 v0) return (P ge0 E0 exp0 v0) with
-      | eval_global_var ge id E v P2 P3 P4 P5 =>
-        Hglobal_var ge id E v P2 P3 P4 P5 (go ge E P2 v P5)
-      | eval_list ge l vs E P3 =>
-        Hlist ge l vs E P3 (go_list ge E l vs P3)
-      | eval_local_var ge id E v P2 => Hlocal_var ge id E v P2
-      | eval_const ge z E => Hconst ge z E
-      end in
-          go ge E expr v eval.
-  *)
+      in
+        match eval in (eager_eval_expr _ TE0 E0 exp0 v0) return (P _ TE0 E0 exp0 v0) with
+        | eager_eval_tuple TE E l vs F2 =>
+          HTuple ge TE E l vs F2 (go_list ge TE E l vs F2)
+        | eval_tuple_sel TE E e l n v eval_e nth =>
+          HTupleSel ge TE E e l n v eval_e (go ge TE E e (stuple l) eval_e) nth
+        | eval_record TE E lp vs F2' =>
+          HRec ge TE E lp vs F2' (go_list ge TE E (map snd lp) vs F2')
+        | eval_record_sel TE E lp str v e eval_e lkup =>
+          HRecordSel ge TE E lp str v e eval_e (go ge TE E e (srec lp) eval_e) lkup
+        | eager_eval_where TE E exp decls v eval_exp =>
+          HWhere ge TE E exp decls v eval_exp (go (bind_decl_groups decls ge) TE (erase_decl_groups decls E) exp v eval_exp)
+        | eager_eval_if TE E c t f v b eval_cond eval_branch =>
+          HIf ge TE E c t f v b eval_cond (go ge TE E c (sbit b) eval_cond) eval_branch (go ge TE E (if b then t else f) v eval_branch)
+        | eager_eval_local_var TE E id v lkupE =>
+          HLocalVar ge TE E id v lkupE
+        | eager_eval_global_var TE E id v exp lkupE lkupge eval_exp =>
+          HGlobalVar ge TE E id v exp lkupE lkupge eval_exp (go ge TE E exp v eval_exp)
+        | eager_eval_abs TE E id exp =>
+          HAbs ge TE E id exp 
+        | eager_eval_tabs TE E e id =>
+          HTAbs ge TE E e id
+        | eager_eval_app TE E f id exp E' TE' a av v eval_clos eval_arg eval_body =>
+          HApp ge TE E f id exp E' TE' a av v eval_clos (go ge TE E f (sclose id exp TE' E') eval_clos)
+               eval_arg (go ge TE E a av eval_arg) eval_body (go ge TE' (extend E' id av) exp v eval_body)
+        | eager_eval_tapp TE TE' E e id e' E' v t te eval_clos eval_targ eval_body =>
+          HTApp ge TE TE' E e id e' E' v t te eval_clos (go ge TE E e (stclose id e' TE' E') eval_clos)
+                eval_targ eval_body (go ge (extend TE' id t) E e' v eval_body)
+        | eager_eval_lazyval v sv TE E seval =>
+          HValue ge v sv TE E seval
+        | eager_eval_list TE E l vs v F2 eqv =>
+          HList ge TE E l vs v F2 (go_list ge TE E l vs F2) eqv
+        | eager_eval_comp TE E llm llidv vs v e epm F2 eqv =>
+          HComp ge TE E llm llidv vs v e epm F2 eqv
+        | eager_eval_builtin TE E l targs args bi v F2types F2not_types bi_sem =>
+          HBuiltin ge TE E l targs args bi v F2types F2not_types (go_list ge TE E (not_types l) args F2not_types) bi_sem
+        end in
+        go ge TE E expr v eval.
+
+Definition eager_eval_expr_ind_useful
+  (P : genv -> tenv -> senv -> Expr -> strictval -> Prop)
+  (HTuple : forall (ge : genv) (TE : tenv) (E : senv) (l : list Expr)
+                   (vs : list strictval),
+      Forall2 (eager_eval_expr ge TE E) l vs ->
+      Forall2 (P ge TE E) l vs ->
+      P ge TE E (ETuple l) (stuple vs))
+  (HTupleSel : forall (ge : genv) (TE : tenv) (E : senv) (e : Expr) 
+                      (l : list strictval) (n : nat) (v : strictval),
+      eager_eval_expr ge TE E e (stuple l) ->
+      P ge TE E e (stuple l) ->
+      nth_error l n = Some v -> P ge TE E (ESel e (TupleSel n)) v)
+  (HRec : forall (ge : genv) (TE : tenv) (E : senv) (l : list (string * Expr))
+                 (vs : list strictval),
+      Forall2 (eager_eval_expr ge TE E) (map snd l) vs ->
+      Forall2 (P ge TE E) (map snd l) vs ->
+      P ge TE E (ERec l) (srec (combine (map fst l) vs)))
+  (HRecordSel : forall (ge : genv) (TE : tenv) (E : senv) (l : list (string * strictval))
+                       (str : string) (v : strictval) (e : Expr),
+      eager_eval_expr ge TE E e (srec l) ->
+      P ge TE E e (srec l) ->
+      lookup str l = Some v -> P ge TE E (ESel e (RecordSel str)) v)
+  (HWhere : forall (ge : genv) (TE : tenv) (E : ident -> option strictval)
+                   (expr : Expr) (decls : list DeclGroup) (v : strictval),
+      eager_eval_expr (bind_decl_groups decls ge) TE 
+                      (erase_decl_groups decls E) expr v ->
+      P (bind_decl_groups decls ge) TE (erase_decl_groups decls E) expr v ->
+      P ge TE E (EWhere expr decls) v)
+  (HIf : forall (ge : genv) (TE : tenv) (E : senv) (c t f : Expr) 
+                (v : strictval) (b : bool),
+      eager_eval_expr ge TE E c (sbit b) ->
+      P ge TE E c (sbit b) ->
+      eager_eval_expr ge TE E (if b then t else f) v ->
+      P ge TE E (if b then t else f) v -> P ge TE E (EIf c t f) v)
+  (HLocalVar : forall (ge : genv) (TE : tenv) (E : ident -> option strictval) 
+                      (id : ident) (v : strictval), E id = Some v -> P ge TE E (EVar id) v)
+  (HGlobalVar : forall (ge : genv) (TE : tenv) (E : ident -> option strictval) 
+                       (id : ident) (v : strictval) (exp : Expr),
+      E id = None ->
+      ge id = Some exp ->
+      eager_eval_expr ge TE E exp v -> P ge TE E exp v -> P ge TE E (EVar id) v)
+  (HAbs : forall (ge : genv) (TE : tenv) (E : senv) (id : ident) (exp : Expr),
+        P ge TE E (EAbs id exp) (sclose id exp TE E))
+  (HTAbs : forall (ge : genv) (TE : tenv) (E : senv) (e : Expr) (id : ident),
+        P ge TE E (ETAbs id e) (stclose id e TE E))
+  (HApp : forall (ge : genv) (TE : tenv) (E : senv) (f : Expr) 
+          (id : ident) (exp : Expr) (E' : ident -> option strictval)
+          (TE' : ident -> option Tval) (a : Expr) (av v : strictval),
+        eager_eval_expr ge TE E f (sclose id exp TE' E') ->
+        P ge TE E f (sclose id exp TE' E') ->
+        eager_eval_expr ge TE E a av ->
+        P ge TE E a av ->
+        eager_eval_expr ge TE' (extend E' id av) exp v ->
+        P ge TE' (extend E' id av) exp v -> P ge TE E (EApp f a) v)
+  (HTApp : forall (ge : genv) (TE : tenv) (TE' : ident -> option Tval) 
+           (E : senv) (e : Expr) (id : ident) (e' : Expr)
+           (E' : ident -> option strictval) (v : strictval) 
+           (t : Tval) (te : Typ),
+         eager_eval_expr ge TE E e (stclose id e' TE' E') ->
+         P ge TE E e (stclose id e' TE' E') ->
+         eager_eval_type ge TE te t ->
+         eager_eval_expr ge (extend TE' id t) E e' v ->
+         P ge (extend TE' id t) E e' v -> P ge TE E (ETApp e (ETyp te)) v)
+  (HValue : forall (ge : genv) (v : val) (sv : strictval) (TE : tenv) (E : senv),
+         strict_eval_val ge v sv -> P ge TE E (EValue v) sv)
+  (HList : forall (ge : genv) (TE : tenv) (E : senv) (l : list Expr)
+           (vs : list strictval) (v : strictval),
+      Forall2 (eager_eval_expr ge TE E) l vs ->
+      Forall2 (P ge TE E) l vs ->
+      v = strict_list vs -> P ge TE E (EList l) v)
+  (HComp : forall (ge : genv) (TE : tenv) (E : senv) (llm : list (list Match))
+                  (llidv : list (list (ident * strictval))) (vs : list strictval)
+                  (v : strictval) (e : Expr),
+      eager_par_match ge TE E llm llidv ->
+      Forall2 (fun senv : senv => eager_eval_expr ge TE senv e)
+              (bind_senvs E llidv) vs ->
+      v = strict_list vs -> P ge TE E (EComp e llm) v)
+  (HBuiltin : forall (ge : genv) (TE : tenv) (E : senv) (l : list Expr)
+           (targs : list Tval) (args : list strictval) 
+           (bi : builtin) (v : strictval),
+      Forall2 (eager_eval_type ge TE) (get_types l) targs ->
+      Forall2 (eager_eval_expr ge TE E) (not_types l) args ->
+      Forall2 (P ge TE E) (not_types l) args ->
+      strict_builtin_sem bi targs args = Some v -> P ge TE E (EBuiltin bi l) v)
+  (ge : genv)
+  (TE : tenv)
+  (E : senv)
+  (expr : Expr)
+  (v : strictval)
+  (eval : eager_eval_expr ge TE E expr v) : P ge TE E expr v .
+Proof.
+  eapply eager_eval_expr_ind_total with (Pl := fun ge TE E => Forall2 (P ge TE E)); try eassumption;
+    intros; econstructor; eauto.
+Defined.
