verif/HMAC_verif.v
@@ -250,7 +250,6 @@ Proof.
           | [ |- _ ] => idtac
           end);
     try (eapply wf_env_name_irrel_GE; eauto).
-  eassumption.
 
   eapply HIDs. simpl. left. reflexivity.
   eapply HIDs. simpl. right. left. reflexivity.
@@ -314,7 +313,6 @@ Proof.
           | [ |- _ ] => idtac
           end);
     try (eapply wf_env_name_irrel_GE; eauto).
-  eassumption.
   
   eapply HIDs. simpl. left. reflexivity.
   eapply HIDs. simpl. right. left. reflexivity.
